Veritas.SeqAux.fsti
@@ -235,7 +235,12 @@ val lemma_reduce_empty (#a:Type) (#b:eqtype) (b0:b) (f:a -> b -> b):
 
 val lemma_reduce_prefix (#a:Type) (#b:eqtype) (b0: b) (f: a -> b -> b) (s: seq a) (i: seq_index s):
   Lemma (reduce b0 f s = reduce (reduce b0 f (prefix s i)) f (suffix s (length s - i)))
-  
+
+val lemma_reduce_property_closure (#a:Type) (#b:eqtype) (p: b -> bool) (b0:b) (f: a -> b -> b) (s: seq a):
+  Lemma (requires (p b0 /\ (forall (x:a). forall (y:b). (p y ==> p (f x y)))))
+        (ensures (p (reduce b0 f s)))
+
 val lemma_reduce_identity (#a:Type) (#b:eqtype) (b0: b) (f: a -> b -> b) (s: seq a):
   Lemma (requires (forall (x:a). f x b0 = b0))
         (ensures (reduce b0 f s = b0))
+
